Cleaned Rust.fst and began BloomFilter

Rust.fst
@@ -1,29 +1,106 @@
 module Rust
 
-let vec (a : Type0) = list a
+module U64 = FStar.UInt64
+module Usize = FStar.UInt32
+module U32 = FStar.UInt32
+module U8 = FStar.UInt8
+module I64 = FStar.Int64
+module Isize = FStar.Int32
+module I32 = FStar.Int32
 
-val length : #a:Type0 -> vec a -> Tot nat
-let length #a v = List.Tot.Base.length v
+type u64 = U64.t
+let _MAX_U64 = FStar.UInt.max_int 64
 
-val fold : #a:Type0 -> #b:Type0 -> (a -> b -> Tot a) -> a -> v:vec b -> Tot a (decreases v)
-let fold #a #b f x v = List.Tot.Base.fold_left f x v
+type usize = Usize.t
+let _MAX_USIZE = FStar.UInt.max_int 32
 
-val index : #a:Type0 -> v:vec a -> i:nat{i < length v} -> Tot a
-let index #a v i = List.Tot.Base.index #a v i
+type u32 = U32.t
+let _MAX_U32 = FStar.UInt.max_int 32
+
+type u8 = U8.t
+let _MAX_U8 = FStar.UInt.max_int 8
+
+type i64 = I64.t
+let _MAX_I64 = FStar.Int.max_int 64
+let _MIN_I64 = FStar.Int.min_int 64
+
+type isize = Isize.t
+let _MAX_ISIZE = FStar.Int.max_int 32
+let _MIN_ISIZE = FStar.Int.min_int 32
+
+type i32 = I32.t
+let _MAX_I32 = FStar.Int.max_int 32
+let _MIN_I32 = FStar.Int.min_int 32
+
+let vec (a : Type0) = l:(list a){List.Tot.Base.length l <= _MAX_USIZE}
+let array (a : Type0) (len: usize) = l:(list a){List.Tot.Base.length l = Usize.v len}
+
+val vec_length : #a:Type0 -> vec a -> Tot usize
+let vec_length #a v = Usize.uint_to_t (List.Tot.Base.length v)
+
+val array_length : #a:Type0 -> #len:usize -> array a len -> Tot usize
+let array_length #a #len array = len
+
+val vec_fold : #a:Type0 -> #b:Type0 -> (a -> b -> Tot a) -> a -> v:vec b -> Tot a (decreases v)
+let vec_fold #a #b f x v = List.Tot.Base.fold_left f x v
+
+val vec_index : #a:Type0 -> vector:vec a -> i:usize{Usize.(i <^ vec_length vector)} -> Tot a
+let vec_index #a v i = List.Tot.Base.index #a v (Usize.v i)
+
+val array_index :
+  #a:Type0 ->
+  #len:usize ->
+  arr:array a len ->
+  i:usize{Usize.(i <^ array_length arr)} ->
+  Tot a
+let array_index #a #len arr i = List.Tot.Base.index #a arr (Usize.v i)
+
+val array_update :
+  #a: Type0 ->
+  #len: usize ->
+  arr: array a len ->
+  i:usize{Usize.(i <^ array_length arr)} ->
+  new_value:a ->
+  Tot (array a len) (decreases arr)
+let rec array_update #a #len arr i new_value =
+   if i = 0ul then
+     (new_value :: (List.Tot.Base.tl arr))
+   else  (List.Tot.Base.hd arr)::(
+     let tail = List.Tot.Base.tl arr in
+     array_update #a #(Usize.(len -^ 1ul)) tail Usize.(i -^ 1ul) new_value
+   )
 
 val enumerate : #a:eqtype -> v:vec a ->
   Tot (vec (a & i:int))
 let enumerate #a v = List.Tot.Base.mapi (fun i e -> (e,i)) v
 
-val foldl :
+private val repeat_left:
+    lo:nat
+  -> hi:nat{lo <= hi}
+  -> a:(i:nat{lo <= i /\ i <= hi} -> Type)
+  -> f:(i:nat{lo <= i /\ i < hi} -> a i -> a (i + 1))
+  -> acc:a lo
+  -> Tot (a hi) (decreases (hi - lo))
+private let rec repeat_left lo hi a f acc =
+  if lo = hi then acc
+  else repeat_left (lo + 1) hi a f (f lo acc)
+
+val vec_foldl :
   #b:Type ->
-  v:vec b{length v > 0} ->
-  a:(i:nat{i < length v} -> Type) ->
-  a 0 ->
-  f:( i:nat{i < length v - 1} -> b -> a i -> Tot (a (i+1))) ->
-  Tot (a (length v - 1)) (decreases v)
-let foldl #b v a x f =
-  Lib.LoopCombinators.repeat_left 0 ((length v - 1))
-    a
-    (fun i acc -> f i (List.Tot.Base.index v i) acc)
+  vector:vec b ->
+  a:(i:usize{Usize.(i <=^ vec_length vector)} -> Type) ->
+  a 0ul ->
+  f:( i:usize{Usize.(i <^ vec_length vector)} -> b -> a i -> Tot (a Usize.(i +^ 1ul))) ->
+  Tot (a (vec_length vector))
+let vec_foldl #b vector a x f =
+  let len = vec_length vector in
+  if len = 0ul then x else
+    repeat_left 0 (Usize.v len)
+    (fun (i:nat{0 <= i /\ i <= Usize.v len}) -> a (Usize.uint_to_t i))
+    (fun i acc -> f (Usize.uint_to_t i) (List.Tot.Base.index vector i) acc)
     x
+
+val vec_all : #b:Type -> vector:vec b -> f:(b -> bool) -> Tot bool (decreases vector)
+let rec vec_all #b vector f = match vector with
+  | [] -> true
+  | hd::tl -> if f hd then vec_all tl f else false
