bloom-filter/BloomFilter.fst
@@ -1,0 +1,146 @@
+module BloomFilter
+
+module U64 = FStar.UInt64
+module Usize = FStar.UInt32
+module U32 = FStar.UInt32
+module U8 = FStar.UInt8
+module I64 = FStar.Int64
+module Isize = FStar.Int32
+module I32 = FStar.Int32
+
+open Rust
+open Spec.BloomFilter
+
+let _BLOOM_HASH_MASK: u32 = 0x00fffffful
+
+let _KEY_SIZE: usize = 12ul
+
+let _ARRAY_SIZE: v:usize{U32.v v = 4096} =
+  let value = Usize.(1ul <<^ _KEY_SIZE) in
+  assert_norm (value = 4096ul);
+  value
+
+let _KEY_MASK: (v:u32{U32.v v = 0xfff}) =
+  let value = Usize.((1ul <<^ _KEY_SIZE) -%^ 1ul) in
+  assert_norm (value = 0xffful);
+  value
+
+noeq type bloom_storage_u8 = {
+  counters: array u8 _ARRAY_SIZE;
+  ghost_state: spec_bloom_storage_u8
+}
+
+
+let valid_index (bf: bloom_storage_u8) = i:usize{Usize.(i <^ array_length bf.counters)}
+
+val hash1: u32 -> r:u32{U32.(r <^ _ARRAY_SIZE)}
+let hash1 hash =
+  let and_value = U32.(hash &^ _KEY_MASK) in
+  admit();//TODO: find how to make F* understand
+  and_value
+
+val hash2: u32 -> r:u32{U32.(r <^ _ARRAY_SIZE)}
+let hash2 hash =
+  let and_value = U32.((hash >>^ _KEY_SIZE) &^ _KEY_MASK) in
+  admit();
+  and_value
+
+let first_slot_index (hash: u32) : r:usize{Usize.(r <^ _ARRAY_SIZE)} =
+  hash1 hash
+
+let second_slot_index (hash: u32) : usize =
+  hash2 hash
+
+val slot_is_empty: bf:bloom_storage_u8 -> valid_index bf -> Tot bool
+let slot_is_empty bf idx =
+  (array_index bf.counters idx) = 0uy
+
+val first_slot_is_empty : bf:bloom_storage_u8 -> u32 -> Tot bool
+let first_slot_is_empty bf hash = slot_is_empty bf (first_slot_index hash)
+
+val second_slot_is_empty : bf:bloom_storage_u8 -> u32 -> Tot bool
+let second_slot_is_empty bf hash = slot_is_empty bf (second_slot_index hash)
+
+val adjust_slot:
+  bf:bloom_storage_u8 ->
+  idx:valid_index bf ->
+  increment:bool{if not increment then not (slot_is_empty bf idx) else true } ->
+  Tot bloom_storage_u8
+let adjust_slot bf idx increment =
+  let slot = array_index bf.counters idx in
+  if slot <> 0xffuy then
+    if increment then
+      { bf with counters = array_update bf.counters idx U8.(slot +^ 1uy) }
+    else
+      { bf with counters = array_update bf.counters idx U8.(slot -^ 1uy) }
+  else bf
+
+val adjust_first_slot:
+  bf:bloom_storage_u8 ->
+  hash:u32 ->
+  increment:bool{if not increment then not (first_slot_is_empty bf hash) else true} ->
+  Tot bloom_storage_u8
+let adjust_first_slot bf hash increment =
+  adjust_slot bf (first_slot_index hash) increment
+
+val adjust_second_slot:
+  bf:bloom_storage_u8 ->
+  hash:u32 ->
+  increment:bool{if not increment then not (second_slot_is_empty bf hash) else true} ->
+  Tot bloom_storage_u8
+let adjust_second_slot bf hash increment =
+  adjust_slot bf (second_slot_index hash) increment
+
+val insert_hash: bf:bloom_storage_u8 -> u32 -> Tot bloom_storage_u8
+let insert_hash bf hash =
+  let bf = adjust_first_slot bf hash true in
+  adjust_second_slot bf hash true
+
+val remove_hash: bf:bloom_storage_u8 -> u32 -> Tot bloom_storage_u8
+let remove_hash bf hash =
+  (* BEGIN ADDED CODE *)
+  (* They never check before substracting in the slots ! Negative overflow might occur *)
+  if (first_slot_is_empty bf hash) then bf else begin
+  (* END ADDED CODE*)
+    let bf = adjust_first_slot bf hash false in
+    (* BEGIN ADDED CODE *)
+    if (second_slot_is_empty bf hash) then adjust_first_slot bf hash true else
+    (* END ADDED CODE *)
+    adjust_second_slot bf hash false
+  end
+
+val might_contain_hash: bf:bloom_storage_u8 -> u32 -> bool
+let might_contain_hash bf hash =
+  not (first_slot_is_empty bf hash) &&
+  not (second_slot_is_empty bf hash)
+
+let rec list_all (l: list element) (f:(element -> bool)) : Tot bool (decreases l) =
+  match l with
+  | [] -> true
+  | hd::tl -> if f hd then list_all tl f else false
+
+let is_valid_bloom_filter (bf: bloom_storage_u8) : Tot bool =
+  let all_elements = bf.ghost_state.elements in
+  list_all all_elements (fun e ->
+    might_contain_hash bf (hash e)
+  )
+
+type valid_bloom_storage_u8 = bf:bloom_storage_u8{is_valid_bloom_filter bf}
+
+val is_zeroed: bf:bloom_storage_u8 -> Tot bool
+let is_zeroed bf =
+  vec_all bf.counters (fun x -> x = 0uy)
+
+#reset-options "--z3rlimit 100"
+
+val insert_element: bf:valid_bloom_storage_u8 -> element -> Tot valid_bloom_storage_u8
+let insert_element bf e =
+  let hash = hash e in
+  let bf = { bf with ghost_state = spec_insert_element bf.ghost_state e } in
+  insert_hash bf hash
+
+val remove_element: bf:valid_bloom_storage_u8 -> element -> Tot valid_bloom_storage_u8
+let remove_element bf e =
+  let hash = hash e in
+  let bf = { bf with ghost_state = spec_remove_element bf.ghost_state e } in
+  remove_hash bf hash
