bloom-filter/Spec.BloomFilter.fst
@@ -1,0 +1,54 @@
+module Spec.BloomFilter
+
+module U64 = FStar.UInt64
+module Usize = FStar.UInt32
+module U32 = FStar.UInt32
+module U8 = FStar.UInt8
+module I64 = FStar.Int64
+module Isize = FStar.Int32
+module I32 = FStar.Int32
+
+open Rust
+
+assume type element: eqtype
+
+assume val hash: element -> u32
+
+noeq type spec_bloom_storage_u8 = {
+   map: FStar.Map.t element nat;
+   elements: list element
+}
+
+val spec_insert_element:
+  bf:spec_bloom_storage_u8 ->
+  e:element ->
+  Tot spec_bloom_storage_u8
+let spec_insert_element bf e =
+  if FStar.Map.contains bf.map e then
+    let old_count = FStar.Map.sel bf.map e in
+    let new_map = FStar.Map.upd bf.map e (old_count + 1) in
+    if old_count = 0 then
+      { map = new_map; elements = e::bf.elements}
+    else
+      {bf with map = new_map }
+  else
+    { map = FStar.Map.upd bf.map e 1; elements = e::bf.elements }
+
+let rec list_remove (#a:eqtype) (l:list a) (e:a) : Tot (list a) (decreases l)=
+  match l with
+  | [] -> l
+  | hd::tl ->
+    let new_tl = list_remove tl e in
+    if hd = e then new_tl else hd::new_tl
+
+val spec_remove_element:
+  bf:spec_bloom_storage_u8 ->
+  e:element ->
+  Tot spec_bloom_storage_u8
+let spec_remove_element bf e =
+  if FStar.Map.contains bf.map e then
+    let old_count = FStar.Map.sel bf.map e in
+    if old_count = 0 then bf else
+      { map = FStar.Map.upd bf.map e (old_count - 1); elements = list_remove bf.elements e }
+  else
+    bf
